RiscvDialect/Functions/add.lean
@@ -29,4 +29,4 @@ def add_64 :=
     llvm.return %0 : i64
   }].denote
 
-  def context :=
+
