RiscvDialect/Instructions/RISCV-testlowering.lean
@@ -1,0 +1,206 @@
+
+import SSA.Core.Tactic
+import SSA.Core.ErasedContext
+import SSA.Core.HVector
+import SSA.Core.EffectKind
+import SSA.Core.Util
+import RiscvDialect.RDialect
+import SSA.Projects.InstCombine.LLVM.PrettyEDSL
+--import SSA.Projects.InstCombine.Refinement
+import SSA.Projects.InstCombine.Tactic
+import SSA.Projects.InstCombine.TacticAuto
+import SSA.Projects.InstCombine.Base
+import SSA.Projects.InstCombine.ForLean
+import Lean
+import SSA.Core.Framework
+import SSA.Core.Tactic
+import SSA.Core.Util
+import SSA.Core.MLIRSyntax.GenericParser
+import SSA.Core.MLIRSyntax.EDSL
+import SSA.Projects.InstCombine.Tactic
+import Mathlib.Tactic.Ring
+import RiscvDialect.Peephole_Optimizations.RiscVRefinement
+import Qq
+import Lean
+import Mathlib.Logic.Function.Iterate
+import SSA.Core.Framework
+import SSA.Core.Tactic
+import SSA.Core.Util
+import SSA.Core.MLIRSyntax.GenericParser
+import SSA.Core.MLIRSyntax.EDSL
+import SSA.Projects.InstCombine.Tactic
+import SSA.Projects.DCE.DCE
+import Mathlib.Tactic.Ring
+open MLIR AST in
+
+open RV64
+open toRISCV
+open DCE
+
+/-- Tthis file contains tools to lowering riscv instructions to other riscv instructions. Also includes a skeleton of
+a verifed lowering from riscv to riscv but where simple just to get familar with how to modell such translations.
+-/
+
+def comSize{Γ : List Ty} (com: Com RV64 Γ .pure .bv ) : Nat :=
+  match com with
+  |Com.ret _ => 1
+  |Com.var _ c' => 1 + comSize c'
+
+
+def transalte (op :toRISCV.Op) : toRISCV.Op :=
+  match op with
+  | .add => .sub
+  | .sub => .add
+  | .mul => .mul
+  | .div => .div
+  | .and => .and
+  | .or => .or
+  | _ => op -- add more operations as needed
+
+def instruction_translation_refinement (e : Expr RV64 Γ .pure .bv) : { e' : Expr RV64 Γ .pure .bv //  e.denote = e'.denote } :=
+  match e with
+  | Expr.mk
+    (.add)
+    (_)
+    (_)
+    (ls)
+    (_) =>  ⟨ Expr.mk
+    (op := toRISCV.Op.add)
+    (eff_le := by constructor)
+    (ty_eq := rfl)
+    (args := ls)
+    (regArgs := .nil), by rfl ⟩
+  | e  => ⟨ e , by rfl ⟩
+
+def instruction (e : Expr RV64 Γ .pure .bv) :  Expr RV64 Γ .pure .bv :=
+  match e with
+  | Expr.mk
+    (.add)
+    (_)
+    (_)
+    (ls)
+    (_) =>  Expr.mk
+    (op := toRISCV.Op.sub)
+    (eff_le := by constructor)
+    (ty_eq := rfl)
+    (args := ls)
+    (regArgs := .nil)
+  | e  =>  e
+
+
+theorem eq_denote {Γ : List Ty}{V :Ctxt.Valuation Γ} {e e' :Expr RV64 Γ .pure .bv} {c' c₁ :  Com RV64 (Ctxt.snoc Γ Ty.bv) EffectKind.pure .bv} (h1: e.denote = e'.denote ) (h2: c'.denote = c₁.denote): (Com.var e c').denote V = (Com.var e' c₁).denote V
+:= by
+  dsimp [Com.denote]
+  rw [h2]
+  rw [h1]
+
+/--this rewrites riscv into the same riscv instruction and is proven to be correct.
+The purpose of this was to understand the strucutre on how to write lowerings that are proven to be correct.
+-/
+
+def loweringR {Γ : Ctxt Ty} (com : Com RV64 Γ .pure .bv)(fuel : Nat) :  { com' :  Com RV64 Γ .pure .bv //  com.denote = com'.denote } :=
+  match com with
+  | Com.ret x  => ⟨ Com.ret x , by rfl ⟩
+  | Com.var (e) c' =>
+  let ⟨c₁, hc₁⟩ := loweringR c' (fuel - 1)
+  have hc₁ : c'.denote = c₁.denote := by
+    exact hc₁
+  let e' := (instruction_translation_refinement e).val
+  let he := (instruction_translation_refinement e).property
+  ⟨Com.var e' c₁ ,
+  by
+    funext V
+    dsimp [Com.denote]
+    rw [hc₁]
+    rw [he]
+    ⟩
+
+def lowering {Γ : Ctxt Ty} (com : Com RV64 Γ .pure .bv):   Com RV64 Γ .pure .bv  :=
+  match com with
+  | Com.ret x  =>  Com.ret x
+  | Com.var (e) c' =>
+      let e' := (instruction e)
+      Com.var (e') (lowering c')
+
+
+--Test examples to see that the lowering actually works.
+def test_lowering2 : Com RV64 [.bv] .pure .bv :=
+  [RV64_com| {
+  ^entry (%0: !i64 ):
+    %1 = "RV64.add" (%0, %0) : ( !i64, !i64 ) -> (!i64)
+    %2 = "RV64.add" (%1, %1) : ( !i64, !i64 ) -> (!i64)
+    %3 = "RV64.add" (%2, %2) : ( !i64, !i64 ) -> (!i64)
+    "return" (%3) : ( !i64) -> ()
+}]
+
+def test_lowering2Result : Com RV64 [.bv] .pure .bv :=
+  [RV64_com| {
+  ^entry (%0: !i64 ):
+    %1 = "RV64.sub" (%0, %0) : ( !i64, !i64 ) -> (!i64)
+    %2 = "RV64.sub" (%1, %1) : ( !i64, !i64 ) -> (!i64)
+    %3 = "RV64.sub" (%2, %2) : ( !i64, !i64 ) -> (!i64)
+    "return" (%3) : ( !i64) -> ()
+}]
+def comSize02 := comSize test_lowering2
+def test_lowering22 : Com RV64 [.bv] .pure .bv := (lowering test_lowering2)
+
+theorem bigLoweringCorrect : test_lowering22 = test_lowering2Result := by
+  unfold test_lowering22 test_lowering2Result  lowering
+  simp
+  native_decide
+
+def test_lowering : Com RV64 [.bv] .pure .bv :=
+  [RV64_com| {
+  ^entry (%0: !i64 ):
+    %1 = "RV64.add" (%0, %0) : ( !i64, !i64 ) -> (!i64)
+    "return" (%1) : ( !i64) -> ()
+}]
+
+def comSize01 := comSize test_lowering
+def test : lowering  [RV64_com| {
+  ^entry (%0: !i64, %2: !i64 ):
+    %1 = "RV64.add" (%0, %0) : ( !i64, !i64 ) -> (!i64)
+    "return" (%1) : ( !i64) -> ()
+}]  =
+  [RV64_com| {
+  ^entry (%reg1: !i64, %reg2: !i64 ):
+    %1 = "RV64.sub" (%reg1, %reg1) : ( !i64, !i64 ) -> (!i64)
+    "return" (%1) : ( !i64) -> ()
+}] := by
+  unfold lowering
+  simp
+  native_decide
+
+def com_eq_IR : [RV64_com| {
+  ^entry (%0: !i64 ):
+    %1 = "RV64.sub" (%0, %0) : ( !i64, !i64 ) -> (!i64)
+    "return" (%1) : ( !i64) -> ()
+}] = Com.var (sub ⟨0, by simp [Ctxt.snoc]⟩ ⟨0, by simp [Ctxt.snoc]⟩) (Com.ret ⟨0, by simp [Ctxt.snoc]⟩) :=
+  by
+  native_decide
+
+def test_explicit :
+  lowering  [RV64_com| {
+  ^entry (%0: !i64 ):
+    %1 = "RV64.add" (%0, %0) : ( !i64, !i64 ) -> (!i64)
+    "return" (%1) : ( !i64) -> ()
+}] = Com.var (sub ⟨0, by simp [Ctxt.snoc]⟩ ⟨0, by simp [Ctxt.snoc]⟩) (Com.ret ⟨0, by simp [Ctxt.snoc]⟩)
+  := by
+  unfold lowering
+  simp
+  unfold instruction
+  native_decide
+
+
+-- TO UNDERSTAND HOW THE CONTEXT MOVES
+def test_explicit_context :
+  lowering  [RV64_com| {
+  ^entry (%0: !i64, %2 : !i64 ): -- context grows from left to right aka gets added from left to right and thus: %0 is index 1 and %2 is index 0
+    %1 = "RV64.add" (%0, %0) : ( !i64, !i64 ) -> (!i64) -- regarding context : left most has highst index
+    "return" (%1) : ( !i64) -> ()
+}] = Com.var (sub ⟨1, by simp [Ctxt.snoc]⟩ ⟨1, by simp [Ctxt.snoc]⟩) (Com.ret ⟨0, by simp [Ctxt.snoc]⟩)
+  := by
+  unfold lowering
+  simp
+  unfold instruction
+  native_decide
