RiscvDialect/Instructions/llvm-to-llvm-lowering.lean
@@ -1,0 +1,31 @@
+import RiscvDialect.RDialect
+import RiscvDialect.RefinementDialect
+import SSA.Projects.InstCombine.LLVM.Semantics
+import SSA.Projects.InstCombine.LLVM.PrettyEDSL
+import SSA.Projects.InstCombine.Refinement
+import SSA.Projects.InstCombine.Tactic
+import SSA.Projects.InstCombine.TacticAuto
+import SSA.Projects.InstCombine.Base
+import SSA.Projects.InstCombine.ForLean
+import RiscvDialect.Instructions.riscv_instructions
+import RiscvDialect.Instructions.llvm_instructions
+import RiscvDialect.Peephole_Optimizations.RISCVRewrites
+import Lean
+
+open LLVM
+
+
+
+/-- this file contains the function to lower llvm instructions into other llvm instructions.
+The purpose of this was to test the design of the translation process. -/
+
+def loweringLLVMToLLVM {Γ : Ctxt LLVM.Ty} (com : Com LLVM Γ .pure (.bitvec 64)) :   Option (Com LLVM Γ .pure (.bitvec 64))  :=
+  match Γ, com with
+  | _, Com.ret x  =>  some (Com.ret x)
+  | _, Com.var (α := InstCombine.Ty.bitvec 64 ) (e) c' =>
+        let e' := (transf e) -- map the expression to a riscv expression
+        match lowering c' with
+        | some com => some (Com.var (e') (com))
+        | none => none
+  | _, Com.var (α := InstCombine.Ty.bitvec _) _ _ =>
+      none
