RiscvDialect/Instructions/llvm_instructions.lean
@@ -1,0 +1,34 @@
+import RiscvDialect.RDialect
+import RiscvDialect.RefinementDialect
+import SSA.Projects.InstCombine.LLVM.Semantics
+import SSA.Projects.InstCombine.LLVM.PrettyEDSL
+import SSA.Projects.InstCombine.Refinement
+import SSA.Projects.InstCombine.Tactic
+import SSA.Projects.InstCombine.TacticAuto
+import SSA.Projects.InstCombine.Base
+import SSA.Projects.InstCombine.ForLean
+import Lean
+
+/-- this file contains a collection of llvm programs that each modell one instruction. 
+
+-/
+
+def llvm_add :=
+  [llvm(64)| {
+^bb0(%X : i64, %Y : i64):
+      %v1 = llvm.add  %X, %Y : i64
+      llvm.return %v1 : i64
+  }]
+
+def llvm_sub :=
+    [llvm(64)| {
+^bb0(%X : i64, %Y : i64):
+      %v1 = llvm.sub  %X, %Y : i64
+      llvm.return %v1 : i64
+  }]
+
+def llvm_ret:=
+  [llvm(64)| {
+    ^bb0(%X : i64):
+    llvm.return %X : i64
+  }]
