RiscvDialect/Instructions/riscv_instructions.lean
@@ -1,0 +1,35 @@
+import RiscvDialect.RDialect
+import RiscvDialect.RefinementDialect
+import SSA.Projects.InstCombine.LLVM.Semantics
+import SSA.Projects.InstCombine.LLVM.PrettyEDSL
+import SSA.Projects.InstCombine.Refinement
+import SSA.Projects.InstCombine.Tactic
+import SSA.Projects.InstCombine.TacticAuto
+import SSA.Projects.InstCombine.Base
+import SSA.Projects.InstCombine.ForLean
+import Lean
+
+open toRISCV
+
+/-- this file contains a collection of RISCV instructions modelled as computations where each computation contains
+one instruction-/
+
+def riscv_add :=
+  [RV64_com| {
+    ^entry (%X: !i64, %Y: !i64):
+    %v1 = "RV64.add" (%X, %Y) : (!i64, !i64) -> (!i64)
+    "return" (%v1) : (!i64, !i64) -> ()
+  }]
+
+def riscv_sub :=
+  [RV64_com| {
+    ^entry (%X: !i64, %Y: !i64):
+    %v1 = "RV64.sub" (%Y, %X ) : (!i64, !i64) -> (!i64)
+    "return" (%v1) : (!i64, !i64) -> ()
+  }]
+
+def rhs_riscv_ret :=
+  [RV64_com| {
+  ^entry (%0 : !i64 ):
+    "return" (%0) : ( !i64 ) -> ()
+}]
