RiscvDialect/Peephole_Optimizations/llvm_riscv.lean
@@ -1,0 +1,205 @@
+import SSA.Core.MLIRSyntax.EDSL
+import SSA.Core.Framework
+import SSA.Core.Util
+import SSA.Core.Util.ConcreteOrMVar
+import SSA.Projects.InstCombine.ForStd
+import SSA.Projects.InstCombine.LLVM.Semantics
+open LLVM
+
+/-- this file is stil in progress and tried to modell riscv and llvm within one context.
+Didnt continue implementing this so far.-/
+
+namespace riscv.semantics
+
+
+def RTYPE_pure64_RISCV_ADD (rs2_val : BitVec 64) (rs1_val : BitVec 64) :BitVec 64 :=
+      BitVec.add rs1_val rs2_val
+
+-- insert the llvm add semantics
+
+end riscv.semantics
+
+namespace llvm.semantics
+
+end llvm.semantics
+
+namespace llvm.riscv
+section Dialect
+
+inductive Op
+|riscv.add
+|llvm.add (nswnuw : NoWrapFlags := {nsw := false, nuw := false} )
+deriving DecidableEq, Repr
+
+
+inductive Ty -- here belongs what my operations operate on
+  | bv64 : Ty
+  | opt64 : Ty
+  -- need to add the llvm option type
+  deriving DecidableEq, Repr
+
+open TyDenote (toType) in
+instance LLVMRISCVTyDenote : TyDenote Ty where
+toType := fun
+| Ty.bv64 => BitVec 64
+| Ty.opt64 => Option (BitVec 64)
+
+abbrev llvm.riscv : Dialect where
+  Op := Op -- define the avaiable operations
+  Ty := Ty -- define the avaiable types
+
+@[simp, reducible]
+def Op.sig : Op → List Ty
+|riscv.add => [Ty.bv64, Ty.bv64]
+|llvm.add _ => [Ty.opt64, Ty.opt64]
+--|llvm.add =>
+
+
+@[simp, reducible] -- reduceable means this expression can always be expanded by the type checker when type checking
+def Op.outTy : Op  → Ty
+|riscv.add => Ty.bv64
+|llvm.add _ => Ty.opt64
+
+@[simp, reducible]
+def Op.signature : Op → Signature (Ty) :=
+  fun o => {sig := Op.sig o, outTy := Op.outTy o, regSig := []}
+
+instance : DialectSignature llvm.riscv := ⟨Op.signature⟩
+
+@[simp, reducible]
+instance : DialectDenote (llvm.riscv) where denote
+  |.riscv.add, regs, _ => riscv.semantics.RTYPE_pure64_RISCV_ADD (regs.getN 0 (by simp [DialectSignature.sig, signature]))  (regs.getN 1 (by simp [DialectSignature.sig, signature]))
+  |.llvm.add flags, regs, _  =>  LLVM.add (regs.getN 0 (by simp [DialectSignature.sig, signature])) (regs.getN 1 (by simp [DialectSignature.sig, signature])) flags
+end Dialect
+
+def riscv.add {Γ : Ctxt _} (e₁ e₂: Ctxt.Var Γ .bv64) : Expr llvm.riscv Γ .pure .bv64  :=
+  Expr.mk
+    (op := llvm.riscv.Op.riscv.add)
+    (eff_le := by constructor)
+    (ty_eq := rfl)
+    (args := .cons e₁ <| .cons e₂ .nil)
+    (regArgs := HVector.nil)
+
+def llvm.add {Γ : Ctxt _} (e₁ e₂: Ctxt.Var Γ .opt64) : Expr llvm.riscv Γ .pure .opt64  :=
+  Expr.mk
+    (op := llvm.riscv.Op.llvm.add)
+    (eff_le := by constructor)
+    (ty_eq := rfl)
+    (args := .cons e₁ <| .cons e₂ .nil)
+    (regArgs := HVector.nil)
+
+def mkTy : MLIR.AST.MLIRType φ → MLIR.AST.ExceptM llvm.riscv llvm.riscv.Ty
+  | MLIR.AST.MLIRType.undefined s => do
+    match s with
+    | "r64" => return .bv64 --maybe change it later
+    | "i64" => return .opt64
+    | _ => throw .unsupportedType
+  | _ => throw .unsupportedType
+
+instance instTransformTy : MLIR.AST.TransformTy llvm.riscv 0 where
+  mkTy := mkTy
+
+
+def mkExpr (Γ : Ctxt _) (opStx : MLIR.AST.Op 0) :
+  MLIR.AST.ReaderM (llvm.riscv) (Σ eff ty, Expr (llvm.riscv) Γ eff ty) := do
+    match opStx.args with
+    | v₁Stx::v₂Stx:: [] =>
+        let ⟨ty₁, v₁⟩ ← MLIR.AST.TypedSSAVal.mkVal Γ v₁Stx
+        let ⟨ty₂, v₂⟩ ← MLIR.AST.TypedSSAVal.mkVal Γ v₂Stx
+        match ty₁, ty₂, opStx.name with
+        | .bv64 , .bv64 , "add" => --refers to an assembly add
+              return ⟨ .pure, .bv64 ,⟨ .riscv.add, by rfl, by constructor,
+               .cons v₁ <| .cons v₂ <| .nil,
+                .nil⟩⟩
+        | .opt64 , .opt64 , "llvm.add" => -- unsure if handeld flags correctly
+              return ⟨ .pure, .opt64 ,⟨ .llvm.add , by rfl, by constructor,
+               .cons v₁ <| .cons v₂ <| .nil,
+                .nil⟩⟩
+        | _ ,_, _ => throw <| .unsupportedOp s!"wrong number of arguemnts, more than 2 arguemnts  {repr opStx}"
+    | _  => throw <| .unsupportedOp "didnt implement instruction yet "
+
+instance : MLIR.AST.TransformExpr (llvm.riscv) 0 where
+  mkExpr := mkExpr
+
+def mkReturn (Γ : Ctxt _) (opStx : MLIR.AST.Op 0) : MLIR.AST.ReaderM (llvm.riscv)
+    (Σ eff ty, Com llvm.riscv Γ eff ty) :=
+  if opStx.name == "return"
+  then match opStx.args with
+  | vStx::[] => do
+    let ⟨ty, v⟩ ← MLIR.AST.TypedSSAVal.mkVal Γ vStx
+    return ⟨.pure, ty, Com.ret v⟩
+  | _ => throw <| .generic s!"Ill-formed return statement (wrong arity, expected 1, got {opStx.args.length})"
+  else throw <| .generic s!"Tried to build return out of non-return statement {opStx.name}"
+
+instance : MLIR.AST.TransformReturn (llvm.riscv) 0 where
+  mkReturn := mkReturn
+
+open Qq MLIR AST Lean Elab Term Meta in
+elab "[_| " reg:mlir_region "]" : term => do
+  SSA.elabIntoCom reg q(llvm.riscv)
+
+end llvm.riscv
+
+
+open llvm.semantics
+open llvm.riscv
+
+
+def exampleLLVM : Com llvm.riscv [.opt64] .pure .opt64 :=
+[_|{
+  ^entry (%0: !i64 ):
+  %1 = "llvm.add" (%0, %0) : (!i64, !i64 ) -> (!i64)
+  "return" (%1) : ( !i64) -> ()
+}]
+
+-- why doesnt it work over a generic list
+def exampleLLVMg {Γ : List llvm.riscv.Ty } : Com llvm.riscv Γ .pure .opt64 :=
+[_|{
+  ^entry (%0: !i64 ):
+  %1 = "llvm.add" (%0, %0) : (!i64, !i64 ) -> (!i64)
+  "return" (%1) : ( !i64) -> ()
+}]
+
+
+def exampleRiscv : Com llvm.riscv [.bv64] .pure .bv64 :=
+[_| {
+  ^entry (%0: !r64 ):
+  %1 = "add" (%0, %0) : (!r64, !r64 ) -> (!r64)
+  "return" (%1) : ( !r64) -> ()
+}]
+
+-- try to modell it as a rewrite but then have the problem of the denotation
+
+
+
+
+
+-- do I need to establish a context mapping or exetend the context Γ
+def instruction (e : Expr llvm.riscv Γ .pure .opt64) :  Expr llvm.riscv Γ .pure .bv64 :=
+  match e with
+  | Expr.mk
+    (.llvm.add)
+    (_)
+    (_)
+    (.cons e₁ <| .cons e₂ <| .nil ) -- are of type .opt64 which are option bitvector -> can either extract them and add them to the context but then need to know
+    (_) =>  Expr.mk
+    (op := .riscv.add)
+    (eff_le := by constructor)
+    (ty_eq := rfl)
+    (args := .cons e₁ <| .cons e₂ <| .nil  )
+    (regArgs := .nil)
+  | e  => e -- still wrong type
+
+-- approach:
+  -- lower it via transforming the expressions
+  -- lower it via modelling the translation as rewrites
+
+
+-- either let them be in the same context and add the riscv version of the varible to the context but then there is the issue of
+-- how do I know which value it has (aka the llvm context would then get eleminated i guess)
+def lowering {Γ Δ : Ctxt Ty} (com : Com llvm.riscv Γ .pure .opt64)(fuel : Nat) :  Com llvm.riscv Δ .pure .bv64  :=
+  match com with
+  | Com.ret x  =>  Com.ret x -- do I now need to know the valuation ? -- extract the variable and add it to the riscv context and then return that
+  | Com.var (e) c' =>
+  let e' := (instruction e)
+  Com.var (e') (lowering c' (fuel - 1))
