RiscvDialect/Peephole_Optimizations/printer.lean
@@ -1,0 +1,11 @@
+import SSA.Core.MLIRSyntax.EDSL
+import SSA.Core.Framework
+import SSA.Core.Util
+import SSA.Core.Util.ConcreteOrMVar
+import SSA.Projects.InstCombine.ForStd
+import SSA.Projects.InstCombine.LLVM.Semantics
+
+
+-- goal is to implement a printer that takes in the Com and Expr and prints the IR back
+
+
